working on new version of MutableBtree

examples/MutableBtree.dfy
@@ -3,20 +3,17 @@ include "../lib/total_order.dfy"
 include "../lib/sequences.dfy"
 include "../lib/Arrays.dfy"
 include "../lib/Maps.dfy"
+include "BtreeSpec.dfy"
 
 abstract module MutableBtree {
   import opened NativeTypes
   import opened Seq = Sequences
   import opened Maps
-  import Arrays
-  import Keys : Total_Order
+  import BS : BtreeSpec
+  
+  type Key = BS.Keys.Element
+  type Value = BS.Value
 
-  type Key = Keys.Element
-  type Value
-    
-  datatype QueryResult =
-    | Found(value: Value)
-    | NotFound
     
   function method MaxKeysPerLeaf() : uint64
     ensures 1 < MaxKeysPerLeaf() as int < Uint64UpperBound() / 2
@@ -27,850 +24,592 @@ abstract module MutableBtree {
   function method DefaultValue() : Value
   function method DefaultKey() : Key
 
-  datatype ImmutableNode =
-    | ImmutableLeaf(keys: seq<Key>, values: seq<Value>)
-    | ImmutableIndex(pivots: seq<Key>, children: seq<ImmutableNode>)
-  
-  function AllKeysNode(node: ImmutableNode) : set<Key>
+  datatype Node =
+    | Leaf(ghost repr: set<object>, nkeys: uint64, keys: array<Key>, values: array<Value>)
+    | Index(ghost repr: set<object>, nchildren: uint64, pivots: array<Key>, children: array<Node>)
+
+  predicate WFShape(node: Node)
+    reads node.repr
+    decreases node.repr
   {
     match node {
-      case ImmutableLeaf(keys, values) => set k | k in keys
-      case ImmutableIndex(pivots, children) => set i, k | 0 <= i < |children| && k in AllKeysNode(children[i]) :: k
+      case Leaf(repr, nkeys, keys, values) =>
+        && keys in repr
+        && values in repr
+        && 0 <= nkeys as int <= MaxKeysPerLeaf() as int == keys.Length
+        && values.Length == keys.Length
+      case Index(repr, nchildren, pivots, children) =>
+        && pivots in repr
+        && children in repr
+        && 0 < nchildren as int <= MaxChildren() as int == children.Length
+        && pivots.Length == MaxChildren() as int - 1
+        && (forall i :: 0 <= i < nchildren ==> children[i].repr < repr)
+        && (forall i {:trigger children[i].repr} :: 0 <= i < nchildren as int ==> pivots !in children[i].repr)
+        && (forall i {:trigger children[i].repr} :: 0 <= i < nchildren as int ==> children !in children[i].repr)
+        && (forall i, j {:trigger children[i].repr, children[j].repr} :: 0 <= i < j < nchildren as int ==> children[i].repr !! children[j].repr)
+        && (forall i :: 0 <= i < nchildren ==> WFShape(children[i]))
+    }
+  }
+
+  function LocalKeys(node: Node) : set<Key>
+    requires WFShape(node)
+    reads node.repr
+  {
+    match node {
+      case Leaf(_, nkeys, keys, _) => set k | k in keys[..nkeys]
+      case Index(_, nchildren, pivots, _) => set i | 0 <= i < nchildren-1 :: pivots[i]
     }    
   }
   
-  predicate WFLeaf(leaf: ImmutableNode)
-    requires leaf.ImmutableLeaf?
+  predicate WFLeaf(node: Node)
+    requires WFShape(node)
+    requires node.Leaf?
+    reads node.repr
   {
-    && |leaf.keys| == |leaf.values|
-    && Keys.IsStrictlySorted(leaf.keys)
+    && BS.Keys.IsStrictlySorted(node.keys[..node.nkeys])
   }
 
-  predicate WFIndex(index: ImmutableNode)
-    requires index.ImmutableIndex?
-    decreases index, 0
+  predicate WFIndex(node: Node)
+    requires WFShape(node)
+    requires node.Index?
+    reads node.repr
+    decreases node.repr, 0
   {
-    && |index.pivots| == |index.children| - 1
-    && Keys.IsStrictlySorted(index.pivots)
-    && (forall i :: 0 <= i < |index.children| ==> WFNode(index.children[i]))
-    && (forall i :: 0 <= i < |index.children| ==> AllKeysNode(index.children[i]) != {})
-    && (forall i, key :: 0 <= i < |index.children|-1 && key in AllKeysNode(index.children[i]) ==> Keys.lt(key, index.pivots[i]))
-    && (forall i, key :: 0 < i < |index.children|   && key in AllKeysNode(index.children[i]) ==> Keys.lte(index.pivots[i-1], key))
+    && BS.Keys.IsStrictlySorted(node.pivots[..node.nchildren-1])
+    && (forall i :: 0 <= i < node.nchildren ==> WF(node.children[i]))
+    && (forall i :: 0 <= i < node.nchildren ==> LocalKeys(node.children[i]) != {})
+    && (forall i, key :: 0 <= i < node.nchildren-1 && key in LocalKeys(node.children[i]) ==> BS.Keys.lt(key, node.pivots[i]))
+    && (forall i, key :: 0 < i < node.nchildren   && key in LocalKeys(node.children[i]) ==> BS.Keys.lte(node.pivots[i-1], key))
   }
 
-  predicate WFNode(node: ImmutableNode)
-    decreases node, 1
-  {
-    match node {
-      case ImmutableLeaf(_, _) =>  WFLeaf(node)
-      case ImmutableIndex(_, _) => WFIndex(node)
-    }
-  }
-
-  function InterpretLeaf(leaf: ImmutableNode) : map<Key, Value>
-    requires leaf.ImmutableLeaf?
-    requires WFLeaf(leaf)
-  {
-    Keys.PosEqLargestLteForAllElts(leaf.keys);
-    map k | (k in leaf.keys) :: leaf.values[Keys.LargestLte(leaf.keys, k)]
-  }
-
-  function InterpretIndex(index: ImmutableNode) : map<Key, Value>
-    requires index.ImmutableIndex?
-    requires WFIndex(index)
-    decreases index, 0
-  {
-    map key |
-      && key in AllKeysNode(index)
-      && key in InterpretNode(index.children[Keys.LargestLte(index.pivots, key) + 1])
-      :: InterpretNode(index.children[Keys.LargestLte(index.pivots, key) + 1])[key]
-  }
-
-  function InterpretNode(node: ImmutableNode) : map<Key, Value>
-    requires WFNode(node)
-    decreases node, 1
+  predicate WF(node: Node)
+    requires WFShape(node)
+    reads node.repr
+    decreases node.repr, 1
   {
     match node {
-      case ImmutableLeaf(_, _) => InterpretLeaf(node)
-      case ImmutableIndex(_, _) => InterpretIndex(node)
+      case Leaf(_, _, _, _) => WFLeaf(node)
+      case Index(_, _, _, _) => WFIndex(node)
     }
   }
 
-  predicate SplitLeaf(oldleaf: ImmutableNode, leftleaf: ImmutableNode, rightleaf: ImmutableNode, pivot: Key)
+  function IndexPrefix(node: Node) : (result: Node)
+    requires WFShape(node)
+    requires WF(node)
+    requires node.Index?
+    requires 1 < node.nchildren
+    reads node.repr
   {
-    && oldleaf.ImmutableLeaf?
-    && leftleaf.ImmutableLeaf?
-    && rightleaf.ImmutableLeaf?
-    && WFLeaf(oldleaf)
-    && WFLeaf(leftleaf)
-    && WFLeaf(rightleaf)
-    && 0 < |leftleaf.keys|
-    && 0 < |rightleaf.keys|
-    && oldleaf.keys == leftleaf.keys + rightleaf.keys
-    && oldleaf.values == leftleaf.values + rightleaf.values
-    && Keys.lt(Last(leftleaf.keys), pivot)
-    && Keys.lte(pivot, rightleaf.keys[0])
+    Index(node.repr - node.children[node.nchildren-1].repr, node.nchildren-1, node.pivots, node.children)
   }
 
-  lemma SplitLeafInterpretation(oldleaf: ImmutableNode, leftleaf: ImmutableNode, rightleaf: ImmutableNode, pivot: Key)
-    requires SplitLeaf(oldleaf, leftleaf, rightleaf, pivot)
-    ensures InterpretLeaf(oldleaf) == MapDisjointUnion(InterpretLeaf(leftleaf), InterpretLeaf(rightleaf))
+  lemma IndexPrefixWF(node: Node)
+    requires WFShape(node)
+    requires WF(node)
+    requires node.Index?
+    requires 1 < node.nchildren
+    ensures WF(IndexPrefix(node))
   {
-    var oldint := InterpretLeaf(oldleaf);
-    var leftint := InterpretLeaf(leftleaf);
-    var rightint := InterpretLeaf(rightleaf);
-    var newint := MapDisjointUnion(leftint, rightint);
-
-    forall key | key in oldint
-      ensures newint[key] == oldint[key]
-    {
-      var llte := Keys.LargestLte(oldleaf.keys, key);
-      if llte < |leftleaf.keys| {
-        Keys.PosEqLargestLte(leftleaf.keys, key, llte);
-      } else {
-        var rightllte := llte - |leftleaf.keys|;
-        Keys.PosEqLargestLte(rightleaf.keys, key, rightllte);
-      }
-    }
+    BS.Keys.reveal_IsStrictlySorted();
   }
   
-  predicate SplitIndex(oldindex: ImmutableNode, leftindex: ImmutableNode, rightindex: ImmutableNode, pivot: Key)
+  function ToImmutableNode(node: Node) : (result: BS.Node)
+    requires WFShape(node)
+    requires WF(node)
+    reads node.repr
+    decreases node.repr
   {
-    && oldindex.ImmutableIndex?
-    && leftindex.ImmutableIndex?
-    && rightindex.ImmutableIndex?
-    && WFIndex(oldindex)
-    && WFIndex(leftindex)
-    && WFIndex(rightindex)
-    && oldindex.pivots == leftindex.pivots + [pivot] + rightindex.pivots
-    && oldindex.children == leftindex.children + rightindex.children
-  }
-
-  lemma SplitIndexInterpretation(oldindex: ImmutableNode, leftindex: ImmutableNode, rightindex: ImmutableNode, pivot: Key)
-    requires SplitIndex(oldindex, leftindex, rightindex, pivot)
-    ensures InterpretIndex(oldindex) == Keys.MapPivotedUnion(InterpretIndex(leftindex), pivot, InterpretIndex(rightindex))
-  {
-    var oldint := InterpretIndex(oldindex);
-    var leftint := InterpretIndex(leftindex);
-    var rightint := InterpretIndex(rightindex);
-    var newint := Keys.MapPivotedUnion(leftint, pivot, rightint);
-
-    Keys.reveal_IsStrictlySorted();
-    Keys.PosEqLargestLte(oldindex.pivots, pivot, |leftindex.pivots|);
-    
-    forall key | key in oldint
-      ensures MapsTo(newint, key, oldint[key])
-    {
-      if Keys.lt(key, pivot) {
-      } else {
-      }
+    match node {
+      case Leaf(_, nkeys, keys, values) => BS.Leaf(keys[..nkeys], values[..nkeys])
+      case Index(repr, nchildren, pivots, children) =>
+        assert WFIndex(node); // FIXME: WFT?  Dafny can't see this in emacs
+        if nchildren == 1 then
+          BS.Index([], [ToImmutableNode(children[0])])
+        else
+          IndexPrefixWF(node);
+          var imprefix := ToImmutableNode(IndexPrefix(node));
+          var imlastchild := ToImmutableNode(children[nchildren-1]);
+          BS.Index(imprefix.pivots + [pivots[nchildren-2]], imprefix.children + [imlastchild])
     }
+  }
 
-    forall key | key in newint
-      ensures MapsTo(oldint, key, newint[key])
-    {
-      if Keys.lt(key, pivot) {
-        var llte := Keys.LargestLte(leftindex.pivots, key);
-        assert oldindex.children[llte+1] == leftindex.children[llte+1];
+  lemma ImmutableWF(node: Node)
+    requires WFShape(node)
+    requires WF(node)
+    ensures BS.WF(ToImmutableNode(node))
+    ensures node.Index? ==> BS.AllKeys(ToImmutableNode(node)) != {}
+    ensures node.Index? ==> ToImmutableNode(node).pivots == node.pivots[..node.nchildren-1]
+    decreases node.repr
+  {
+    if node.Leaf? {
+    } else if node.nchildren == 1 {
+      var imnode := ToImmutableNode(node);
+      if imnode.children[0].Leaf? {
+        assert imnode.children[0].keys[0] in BS.AllKeys(imnode.children[0]);
       } else {
-        var llte := Keys.LargestLte(rightindex.pivots, key);
-        assert oldindex.children[|leftindex.children| + llte + 1] == rightindex.children[llte+1];
+        ImmutableWF(node.children[0]);
       }
-    }
-    
-  }
-  
-  predicate SplitNode(oldnode: ImmutableNode, leftnode: ImmutableNode, rightnode: ImmutableNode, pivot: Key)
-  {
-    || SplitLeaf(oldnode, leftnode, rightnode, pivot)
-    || SplitIndex(oldnode, leftnode, rightnode, pivot)
-  }
-
-  lemma SplitNodeInterpretation(oldnode: ImmutableNode, leftnode: ImmutableNode, rightnode: ImmutableNode, pivot: Key)
-    requires SplitNode(oldnode, leftnode, rightnode, pivot)
-    ensures InterpretNode(oldnode) == Keys.MapPivotedUnion(InterpretNode(leftnode), pivot, InterpretNode(rightnode))
-  {
-    if SplitLeaf(oldnode, leftnode, rightnode, pivot) {
-      SplitLeafInterpretation(oldnode, leftnode, rightnode, pivot);
     } else {
-      SplitIndexInterpretation(oldnode, leftnode, rightnode, pivot);
+      IndexPrefixWF(node);
+      var imprefix := ToImmutableNode(IndexPrefix(node));
+      ImmutableWF(IndexPrefix(node));
+      var imlastchild := ToImmutableNode(node.children[node.nchildren-1]);
+      var imnode := BS.Index(imprefix.pivots + [node.pivots[node.nchildren-2]], imprefix.children + [imlastchild]);
+      assert imnode.pivots == node.pivots[..node.nchildren-1];
+      assert BS.LocalKeys(Last(imnode.children)) == LocalKeys(node.children[node.nchildren-1]);
+    }
+  }
+
+  lemma ImmutableChildIndices(node: Node)
+    requires WFShape(node)
+    requires WF(node)
+    requires node.Index?
+    ensures |ToImmutableNode(node).children| == node.nchildren as int
+    ensures forall i :: 0 <= i < node.nchildren ==>
+           ToImmutableNode(node).children[i] == ToImmutableNode(node.children[i])
+    decreases node.repr
+  {
+    if node.nchildren == 1 {
+    } else {
+      IndexPrefixWF(node);
     }
   }
   
-  predicate SplitChildOfIndex(oldindex: ImmutableNode, newindex: ImmutableNode, childidx: int)
+  function Interpretation(node: Node) : map<Key, Value>
+    requires WFShape(node)
+    requires WF(node)
+    reads node.repr
+    decreases node.repr
   {
-    && oldindex.ImmutableIndex?
-    && newindex.ImmutableIndex?
-    && WFNode(oldindex)
-    && WFNode(newindex)
-    && 0 <= childidx < |oldindex.children|
-    && |newindex.children| == |oldindex.children| + 1 // FIXME: WTF?  Dafny can't get these from WFNode?
-    && |newindex.pivots| == |oldindex.pivots| + 1
-    && |oldindex.pivots| == |oldindex.children| - 1
-    && newindex.pivots == Seq.insert(oldindex.pivots, newindex.pivots[childidx], childidx)
-    && SplitNode(oldindex.children[childidx], newindex.children[childidx], newindex.children[childidx+1], newindex.pivots[childidx])
-    && newindex.children == oldindex.children[..childidx] + [newindex.children[childidx], newindex.children[childidx+1]] + oldindex.children[childidx+1..]
+    ImmutableWF(node);
+    BS.InterpretNode(ToImmutableNode(node))
   }
-
-  lemma SplitChildOfIndexPreservesInterpretation(oldindex: ImmutableNode, newindex: ImmutableNode, childidx: int)
-    requires SplitChildOfIndex(oldindex, newindex, childidx)
-    ensures InterpretNode(newindex) == InterpretNode(oldindex)
+  
+  method QueryLeaf(node: Node, needle: Key) returns (result: BS.QueryResult)
+    requires WFShape(node)
+    requires WF(node)
+    requires node.Leaf?
+    ensures needle in Interpretation(node) ==> result == BS.Found(Interpretation(node)[needle])
+    ensures needle !in Interpretation(node) ==> result == BS.NotFound
+    decreases node.repr, 0
   {
-    var newint := InterpretNode(newindex);
-    var oldint := InterpretNode(oldindex);
-
-    // WTF?  Dafny can't see these (from emacs flycheck mode)
-    assert WFIndex(oldindex);
-    assert WFIndex(newindex);
-    assert oldint == InterpretIndex(oldindex);
-    assert newint == InterpretIndex(newindex);
-    
-    var oldchild := oldindex.children[childidx];
-    var leftchild := newindex.children[childidx];
-    var rightchild := newindex.children[childidx+1];
-    var pivot := newindex.pivots[childidx];
-    SplitNodeInterpretation(oldchild, leftchild, rightchild, pivot);        
-    
-    forall key | key in oldint
-      ensures key in newint && newint[key] == oldint[key]
-    {
-      var llte := Keys.LargestLte(oldindex.pivots, key);
-      if llte + 1 < childidx {
-        assert llte == Keys.LargestLte(newindex.pivots, key);
-      } else if llte + 1 == childidx {
-      } else {
-        var newllte := llte + 1;
-        assert newllte == Keys.LargestLte(newindex.pivots, key);
-        assert newindex.children[newllte+1] == oldindex.children[llte+1];
-      }
-    }
-
-    forall key | key in newint
-      ensures key in oldint
-    {
-      var llte := Keys.LargestLte(newindex.pivots, key);
-      if llte + 1 < childidx {
-        assert llte == Keys.LargestLte(oldindex.pivots, key);
-      } else if llte + 1 == childidx {
-        var oldllte := llte;
-        assert oldllte == Keys.LargestLte(oldindex.pivots, key);
-        assert key in InterpretNode(oldindex.children[Keys.LargestLte(oldindex.pivots, key) + 1]);
-      } else if llte + 1 == childidx + 1 {
-        var oldllte := llte - 1;
-        assert oldllte == Keys.LargestLte(oldindex.pivots, key);
-        assert key in InterpretNode(oldindex.children[Keys.LargestLte(oldindex.pivots, key) + 1]);
-      } else {
-        assert llte - 1 == Keys.LargestLte(oldindex.pivots, key);
-      }
-    }
-  }
-    
-  function InsertLeaf(leaf: ImmutableNode, key: Key, value: Value) : (result: ImmutableNode)
-    requires leaf.ImmutableLeaf?
-    requires WFLeaf(leaf)
-    ensures result.ImmutableLeaf?
-    ensures WFLeaf(result)
-  {
-    var llte := Keys.LargestLte(leaf.keys, key);
-    if 0 <= llte && leaf.keys[llte] == key then
-      ImmutableLeaf(leaf.keys, leaf.values[llte := value])
-    else
-      Keys.strictlySortedInsert(leaf.keys, key, llte);
-      ImmutableLeaf(Seq.insert(leaf.keys, key, llte+1), Seq.insert(leaf.values, value, llte+1))
-  }
-
-  lemma InsertLeafIsCorrect(leaf: ImmutableNode, key: Key, value: Value, result: ImmutableNode)
-    requires leaf.ImmutableLeaf?
-    requires WFLeaf(leaf)
-    requires result == InsertLeaf(leaf, key, value)
-    ensures InterpretNode(result) == InterpretNode(leaf)[key := value]
-  {
-    var llte := Keys.LargestLte(leaf.keys, key);
-    if 0 <= llte && leaf.keys[llte] == key {
-      assert InterpretNode(result) == InterpretNode(leaf)[key := value];
+    var posplus1: uint64 := BS.Keys.ArrayLargestLtePlus1(node.keys, 0, node.nkeys, needle);
+    if 1 <= posplus1 && node.keys[posplus1-1] == needle {
+      result := BS.Found(node.values[posplus1-1]);
     } else {
-      Keys.reveal_IsStrictlySorted();
-      forall k | k in InterpretNode(result).Keys
-        ensures k in InterpretNode(leaf).Keys + {key}
-      {
-        var kpos := IndexOf(result.keys, k);
-        if llte + 1 < kpos {
-          assert k == leaf.keys[kpos-1];
-        }
+      result := BS.NotFound;
+    }
+  }
+
+  method QueryIndex(node: Node, needle: Key) returns (result: BS.QueryResult)
+    requires WFShape(node)
+    requires WF(node)
+    requires node.Index?
+    ensures needle in Interpretation(node) ==> result == BS.Found(Interpretation(node)[needle])
+    ensures needle !in Interpretation(node) ==> result == BS.NotFound
+    decreases node.repr, 0
+  {
+    var posplus1 := BS.Keys.ArrayLargestLtePlus1(node.pivots, 0, node.nchildren-1, needle);
+    result := Query(node.children[posplus1], needle);
+
+    ghost var imnode := ToImmutableNode(node);
+    ImmutableWF(node);
+    ImmutableChildIndices(node);
+    if needle in Interpretation(node) {
+      //assert needle in BS.InterpretNode(imnode);
+      //assert imnode.Index?;
+      assert needle in BS.InterpretIndex(imnode);
+      //assert posplus1 as int == BS.Keys.LargestLte(imnode.pivots, needle) + 1;
+      //assert needle in BS.InterpretNode(imnode.children[posplus1]);
+      //assert BS.InterpretNode(imnode)[needle] == BS.InterpretNode(imnode.children[posplus1])[needle];
+      //assert imnode.children[posplus1] == ToImmutableNode(node.children[posplus1]);
+      //assert needle in Interpretation(node.children[posplus1]);
+    } else {
+      assert needle !in BS.InterpretIndex(imnode);
+      //assert needle !in BS.AllKeys(imnode) || needle !in BS.InterpretNode(imnode.children[posplus1]);
+      //BS.AllKeysIsConsistentWithInterpretationUniversal(imnode);
+      if needle !in BS.AllKeys(imnode) {
+        assert needle !in BS.AllKeys(imnode.children[posplus1]);
       }
+      assert needle !in BS.InterpretNode(imnode.children[posplus1]);
     }
   }
-   
-  trait Node {
-    ghost var subtreeObjects: set<object>
-      
-    predicate WF()
-      ensures WF() ==> this in subtreeObjects
-      reads this, subtreeObjects
-      decreases subtreeObjects, 0
-      
-    function ToImmutableNode() : (imnode: ImmutableNode)
-      requires WF()
-      ensures WFNode(imnode)
-      reads this, subtreeObjects
-      decreases subtreeObjects, 2
-      
-    function AllKeys() : set<Key>
-      requires WF()
-      reads this, subtreeObjects
-      decreases subtreeObjects, 3
-    {
-      AllKeysNode(ToImmutableNode())
+
+  method Query(node: Node, needle: Key) returns (result: BS.QueryResult)
+    requires WFShape(node)
+    requires WF(node)
+    ensures needle in Interpretation(node) ==> result == BS.Found(Interpretation(node)[needle])
+    ensures needle !in Interpretation(node) ==> result == BS.NotFound
+    decreases node.repr, 1
+  {
+    match node {
+      case Leaf(_, _, _, _) => result := QueryLeaf(node, needle);
+      case Index(_, _, _, _) => result := QueryIndex(node, needle);
     }
-
-    function Interpretation() : map<Key, Value>
-      requires WF()
-      reads this, subtreeObjects
-      decreases subtreeObjects, 4
-    {
-      InterpretNode(ToImmutableNode())
-    }
-    
-    // method Query(needle: Key) returns (result: QueryResult)
-    //   requires WF()
-    //   ensures needle in Interpretation() ==> result == Found(Interpretation()[needle])
-    //   ensures needle !in Interpretation() ==> result == NotFound
-    //   decreases subtreeObjects
-
-    // predicate method Full()
-    //   requires WF()
-    //   reads this, subtreeObjects
-      
-    // predicate SplitEnsures(oldint: map<Key, Value>, pivot: Key, rightnode: Node)
-    //   reads this, subtreeObjects
-    //   reads rightnode, rightnode.subtreeObjects
-    // {
-    //   && WF()
-    //   && !Full()
-    //   && rightnode.WF()
-    //   && !rightnode.Full()
-    //   && SplitNode(old(ToImmutableNode()), 
-    //   && Keys.MapPivotedUnion(Interpretation(), pivot, rightnode.Interpretation()) == oldint
-    //   && AllKeys() != {}
-    //   && rightnode.AllKeys() != {}
-    //   && (forall key :: key in AllKeys() ==> Keys.lt(key, pivot))
-    //   && (forall key :: key in rightnode.AllKeys() ==> Keys.lte(pivot, key))
-    // }
-      
-    // method Split() returns (pivot: Key, rightnode: Node)
-    //   requires WF()
-    //   requires Full()
-    //   ensures WF()
-    //   ensures rightnode.WF()
-    //   ensures SplitNode(old(ToImmutableNode()), ToImmutableNode(), rightnode.ToImmutableNode(), pivot)
-    //   ensures !Full()
-    //   ensures !rightnode.Full()
-    //   ensures subtreeObjects <= old(subtreeObjects)
-    //   ensures subtreeObjects !! rightnode.subtreeObjects
-    //   ensures fresh(rightnode.subtreeObjects - old(subtreeObjects))
-    //   modifies this
-
-    // method Insert(key: Key, value: Value)
-    //   requires WF()
-    //   requires !Full()
-    //   ensures WF()
-    //   ensures Interpretation() == old(Interpretation())[key := value]
-    //   ensures AllKeys() == old(AllKeys()) + {key}
-    //   ensures fresh(subtreeObjects-old(subtreeObjects))
-    //   modifies this, subtreeObjects
-    //   decreases AllKeys()
-      
   }
-
-  datatype NodeBox = NodeBox(node: Node?)
-
-  class Leaf extends Node {
-    var nkeys : uint64
-    var keys: array<Key>
-    var values: array<Value>
-
-    predicate WF()
-      ensures WF() ==> this in subtreeObjects
-      reads this, subtreeObjects
-      decreases subtreeObjects, 0
-    {
-      && subtreeObjects == {this, keys, values}
-      && keys != values
-      && keys.Length == MaxKeysPerLeaf() as int
-      && values.Length == MaxKeysPerLeaf() as int
-      && 0 <= nkeys as int <= keys.Length
-      && Keys.IsStrictlySorted(keys[..nkeys])
-    }
-
-    function ToImmutableNode() : (result: ImmutableNode)
-      requires WF()
-      ensures WFNode(result)
-      //ensures result.ImmutableLeaf?
-      reads this, subtreeObjects
-      decreases subtreeObjects, 2
-    {
-      ImmutableLeaf(keys[..nkeys], values[..nkeys])
-    }
     
-    // method Query(needle: Key) returns (result: QueryResult)
-    //   requires WF()
-    //   ensures needle in Interpretation() ==> result == Found(Interpretation()[needle])
-    //   ensures needle !in Interpretation() ==> result == NotFound
-    //   decreases subtreeObjects
-    // {
-    //   //Keys.reveal_IsStrictlySorted();
-    //   var posplus1: uint64 := Keys.ArrayLargestLtePlus1(keys, 0, nkeys, needle);
-    //   if 1 <= posplus1 && keys[posplus1-1] == needle {
-    //     result := Found(values[posplus1-1]);
-    //   } else {
-    //     result := NotFound;
-    //   }
-    // }
-
-    // predicate method Full()
-    //   requires WF()
-    //   reads this, subtreeObjects
-    // {
-    //   nkeys >= MaxKeysPerLeaf()
-    // }
-    
-    // method Split() returns (pivot: Key, rightnode: Node)
-    //   requires WF()
-    //   requires Full()
-    //   ensures WF()
-    //   ensures rightnode.WF()
-    //   ensures SplitNode(old(ToImmutableNode()), ToImmutableNode(), rightnode.ToImmutableNode(), pivot)
-    //   ensures !Full()
-    //   ensures !rightnode.Full()
-    //   ensures subtreeObjects <= old(subtreeObjects)
-    //   ensures subtreeObjects !! rightnode.subtreeObjects
-    //   ensures fresh(rightnode.subtreeObjects - old(subtreeObjects))
-    //   modifies this
-    // {
-    //   var right := new Leaf();
-    //   var boundary := nkeys/2;
-    //   Arrays.Memcpy(right.keys, 0, keys[boundary..nkeys]); // FIXME: remove conversion to seq
-    //   Arrays.Memcpy(right.values, 0, values[boundary..nkeys]); // FIXME: remove conversion to seq
-    //   right.nkeys := nkeys - boundary;
-    //   nkeys := boundary;
-    //   pivot := right.keys[0];
-    //   rightnode := right;
-
-    //   assert keys[..nkeys] == old(keys[..nkeys])[..nkeys];
-    //   Keys.StrictlySortedSubsequence(old(keys[..nkeys]), 0, nkeys as int);
-    //   assert right.keys[..right.nkeys] == old(keys[..nkeys])[boundary..old(nkeys)];
-    //   Keys.StrictlySortedSubsequence(old(keys[..nkeys]), boundary as int, old(nkeys) as int);
-    //   Keys.reveal_IsStrictlySorted();
-    //   assert SplitLeaf(old(ToImmutableNode()), ToImmutableNode(), rightnode.ToImmutableNode(), pivot);
-    // }
-      
-    // method Insert(key: Key, value: Value)
-    //   requires WF()
-    //   requires !Full()
-    //   ensures WF()
-    //   ensures Interpretation() == old(Interpretation())[key := value]
-    //   ensures AllKeys() == old(AllKeys()) + {key}
-    //   ensures fresh(subtreeObjects-old(subtreeObjects))
-    //   modifies this, subtreeObjects
-    //   decreases AllKeys()
-    // {
-    //   var posplus1 := Keys.ArrayLargestLtePlus1(keys, 0, nkeys, key);
-
-    //   if 1 <= posplus1 && keys[posplus1-1] == key {
-    //     values[posplus1-1] := value;
-    //   } else {
-    //     ghost var oldkeys := keys[..nkeys];
-    //     Arrays.Insert(keys, nkeys, key, posplus1);
-    //     Arrays.Insert(values, nkeys, value, posplus1);
-    //     nkeys := nkeys + 1;
-
-    //     InsertMultiset(oldkeys, key, posplus1 as int); // OBSERVE
-    //     Keys.strictlySortedInsert(oldkeys, key, posplus1 as int - 1); // OBSERVE
-    //     Keys.PosEqLargestLte(keys[..nkeys], key, posplus1 as int);
-    //     forall key' |  key' != key && key' in old(Interpretation())
-    //       ensures key' in Interpretation() && Interpretation()[key'] == old(Interpretation())[key']
-    //     {
-    //       var i: int := Keys.LargestLte(old(keys[..nkeys]), key');
-    //       //assert 0 <= i;
-    //       if i < posplus1 as int {
-    //         //assert keys[i] == key';
-    //         Keys.PosEqLargestLte(keys[..nkeys], key', i);
-    //       } else {
-    //         //assert keys[i+1] == key';
-    //         Keys.PosEqLargestLte(keys[..nkeys], key', i+1);
-    //       }
-    //     }
-    //     forall key' | key' != key && key' in Interpretation()
-    //       ensures key' in old(Interpretation()) && old(Interpretation())[key'] == Interpretation()[key']
-    //     {
-    //       var i: int := Keys.LargestLte(keys[..nkeys], key');
-    //       if i < posplus1 as int {
-    //         Keys.PosEqLargestLte(old(keys[..nkeys]), key', i);
-    //       } else {
-    //         Keys.PosEqLargestLte(old(keys[..nkeys]), key', i-1);
-    //       }
-    //     }
-    //   }
-    // }
-
-    // constructor()
-    //   ensures WF()
-    //   ensures Interpretation() == map[]
-    //   ensures !Full()
-    //   ensures fresh(keys)
-    //   ensures fresh(values)
-    // {
-    //   nkeys := 0;
-    //   keys := new Key[MaxKeysPerLeaf()](_ => DefaultKey());
-    //   values := new Value[MaxKeysPerLeaf()](_ => DefaultValue());
-    //   subtreeObjects := {this, keys, values};
-    // }
-  }
-
-  class Index extends Node {
-    var nchildren: uint64
-    var pivots: array<Key>
-    var children: array<NodeBox>
-
-    predicate WF()
-      ensures WF() ==> this in subtreeObjects
-      reads this, subtreeObjects
-      decreases subtreeObjects, 0
-    {
-      && {this, pivots, children} <= subtreeObjects
-      && pivots.Length == (MaxChildren() as int) - 1
-      && children.Length == MaxChildren() as int
-      && 1 < nchildren <= MaxChildren()
-      && (forall i :: 0 <= i < nchildren ==> children[i].node != null)
-      && (forall i :: 0 <= i < nchildren ==> children[i].node in subtreeObjects)
-      && (forall i {:trigger children[i].node.subtreeObjects} :: 0 <= i < nchildren as int ==> children[i].node.subtreeObjects < subtreeObjects)
-      && (forall i {:trigger children[i].node.subtreeObjects} :: 0 <= i < nchildren as int ==> {this, pivots, children} !! children[i].node.subtreeObjects)
-      && (forall i, j {:trigger children[i].node.subtreeObjects, children[j].node.subtreeObjects} :: 0 <= i < j < nchildren as int ==> children[i].node.subtreeObjects !! children[j].node.subtreeObjects)
-      
-      && Keys.IsStrictlySorted(pivots[..nchildren-1])
-      && (forall i :: 0 <= i < nchildren ==> children[i].node.WF())
-      && (forall i :: 0 <= i < nchildren ==> children[i].node.AllKeys() != {})
-      && (forall i, key :: 0 <= i < nchildren-1 && key in children[i].node.AllKeys() ==> Keys.lt(key, pivots[i]))
-      && (forall i, key :: 0 < i < nchildren   && key in children[i].node.AllKeys() ==> Keys.lte(pivots[i-1], key))
-    }
-
-    // static function SeqSubtreeObjects(nodes: seq<NodeBox>) : (result: set<object>)
-    //   requires forall i :: 0 <= i < |nodes| ==> nodes[i].node != null
-    //   reads set i | 0 <= i < |nodes| :: nodes[i].node
-    // {
-    //   set i, o | 0 <= i < |nodes| && o in nodes[i].node.subtreeObjects :: o
-    // }
-
-    // lemma SeqSubtreeObjectsDecreasing()
-    //   requires WF()
-    //   requires 1 < nchildren
-    //   ensures forall i :: 0 <= i < nchildren ==> children[i].node.subtreeObjects < SeqSubtreeObjects(children[..nchildren])
-    //   decreases subtreeObjects, 1
-    // {
-    //   forall i | 0 <= i < nchildren
-    //     ensures children[i].node.subtreeObjects < SeqSubtreeObjects(children[..nchildren])
-    //   {
-    //     if 0 < i {
-    //       assert children[i-1].node.WF();
-    //       assert children[i-1].node !in children[i].node.subtreeObjects;
-    //     } else {
-    //       assert children[i+1].node.WF();
-    //       assert children[i+1].node !in children[i].node.subtreeObjects;
-    //     }
-    //   }
-    // }
-    
-    // static function SeqToImmutableNodeSeq(nodes: seq<NodeBox>) : (result: seq<ImmutableNode>)
-    //   requires forall i :: 0 <= i < |nodes| ==> nodes[i].node != null
-    //   requires forall i :: 0 <= i < |nodes| ==> nodes[i].node.subtreeObjects < SeqSubtreeObjects(nodes)
-    //   requires forall i :: 0 <= i < |nodes| ==> nodes[i].node.WF()
-    //   reads set i | 0 <= i < |nodes| :: nodes[i].node
-    //   reads SeqSubtreeObjects(nodes)
-    //   decreases SeqSubtreeObjects(nodes)
-    // {
-    //   if nodes == [] then
-    //     []
-    //   else
-    //     assert Last(nodes).node.subtreeObjects < SeqSubtreeObjects(nodes);
-    //     SeqToImmutableNodeSeq(DropLast(nodes)) + [Last(nodes).node.ToImmutableNode()]
-    // }
-    
-    function ToImmutableNode() : (imnode: ImmutableNode)
-      requires WF()
-      ensures WFNode(imnode)
-      reads this, subtreeObjects
-      decreases subtreeObjects, 2
-    // {
-    //   var impivots := pivots[..nchildren-1];
-    //   SeqSubtreeObjectsDecreasing();
-    //   assert SeqSubtreeObjects(children[..nchildren]) < subtreeObjects;
-    //   var imchildren := SeqToImmutableNodeSeq(children[..nchildren]);
-    //   ImmutableIndex(impivots, imchildren)
-    // }
-    
-    // lemma AllKeysStrictlyDecreasing()
-    //   requires WF()
-    //   ensures forall i :: 0 <= i < nchildren ==> children[i].node.allKeys < allKeys
-    // {
-    //   forall i | 0 <= i < nchildren
-    //     ensures children[i].node.allKeys < allKeys
-    //   {
-    //     var i' := if i < nchildren-1 then i+1 else 0;
-    //     assert i' != i;
-    //     assert children[i].node.allKeys !! children[i'].node.allKeys;
-    //     assert children[i].node.allKeys <= 
-    //     assert children[i].node.allKeys <= allKeys;
-    //   }
-    // }
-    
-    // method Query(needle: Key) returns (result: QueryResult)
-    //   requires WF()
-    //   ensures needle in Interpretation() ==> result == Found(Interpretation()[needle])
-    //   ensures needle !in Interpretation() ==> result == NotFound
-    //   // ensures result == QueryDef(needle)
-    //   decreases subtreeObjects
-    // {
-    //   var posplus1 := Keys.ArrayLargestLtePlus1(pivots, 0, nchildren-1, needle);
-    //   result := children[posplus1].node.Query(needle);
-    // }
-
-    // predicate method Full()
-    //   requires WF()
-    //   reads this, subtreeObjects
-    // {
-    //   nchildren == MaxChildren()
-    // }
-
-    // method SplitChild(key: Key, childidx: uint64)
-    //   requires WF()
-    //   requires !Full()
-    //   requires childidx as int == 1 + Keys.LargestLte(pivots[..nchildren-1], key)
-    //   requires children[childidx].node.Full()
-    //   ensures WF()
-    //   //ensures Interpretation() == old(Interpretation())
-    //   ensures SplitChildOfIndex(old(ToImmutableNode()), ToImmutableNode(), childidx as int)
-    //   ensures fresh(subtreeObjects-old(subtreeObjects))
-    //   modifies this, pivots, children, children[childidx].node
-    // {
-    //   ghost var oldchildren := children;
-      
-    //   var pivot, right := children[childidx].node.Split();
-    //   Arrays.Insert(pivots, nchildren - 1, pivot, childidx);
-    //   Arrays.Insert(children, nchildren, NodeBox(right), childidx + 1);
-    //   nchildren := nchildren + 1;
-    //   subtreeObjects := subtreeObjects + right.subtreeObjects;
-
-      
-    //   // Keys.LargestLteIsUnique(old(pivots[..nchildren-1]), pivot, childidx as int - 1);
-    //   // Keys.strictlySortedInsert(old(pivots[..nchildren-1]), pivot, childidx as int - 1);
-
-    //   assert forall i: uint64 :: 0 <= i < childidx ==> children[i] == oldchildren[i];
-    //   assert children[childidx as int + 1].node == right;
-    //   assert forall i: uint64 :: childidx + 1 < i < nchildren ==> children[i] == oldchildren[i-1];
-    //   // forall i: int, j: int {:trigger children[i].node.subtreeObjects, children[j].node.subtreeObjects}
-    //   // | 0 <= i < j < nchildren as int
-    //   //   ensures children[i].node.subtreeObjects !! children[j].node.subtreeObjects
-    //   // {
-    //   //   if                                   j  < childidx as int {
-    //   //   } else if                            j == childidx as int {
-    //   //   } else if i  < childidx as int     && j == childidx as int + 1 {
-    //   //   } else if i == childidx as int     && j == childidx as int + 1 {
-    //   //   } else if i  < childidx as int     && j  > childidx as int + 1 {
-    //   //   } else if i == childidx as int     && j  > childidx as int + 1 {
-    //   //   } else if i == childidx as int + 1 && j  > childidx as int + 1 {
-    //   //   } else {
-    //   //   }
-    //   // }
-    //   // // forall i: int, key | 0 <= i < (nchildren as int)-1 && key in children[i].node.allKeys
-    //   // //   ensures Keys.lt(key, pivots[i])
-    //   // // {
-    //   // //   if childidx as int + 1 < i {
-    //   // //     assert children[i] == old(children[i-1]);
-    //   // //   }
-    //   // // }
-    //   // // forall i: int, key | 0 < i < nchildren as int && key in children[i].node.allKeys
-    //   // //   ensures Keys.lt(pivots[i-1], key)
-    //   // // {
-    //   // //   if i < childidx as int {
-    //   // //     assert Keys.lt(pivots[i-1], key);
-    //   // //   } else if i == childidx as int {
-    //   // //     assert Keys.lt(pivots[i-1], key);
-    //   // //   } else if i == childidx as int + 1 {
-    //   // //     assert Keys.lt(pivots[i-1], key);
-    //   // //   } else {
-    //   // //     assert Keys.lt(pivots[i-1], key);
-    //   // //   }
-    //   // // }
-    //   // assert WF();
-        
-    //   // forall key | key in old(Interpretation())
-    //   //   ensures key in Interpretation() && Interpretation()[key] == old(Interpretation()[key])
-    //   // {
-    //   //   var llte: int := Keys.LargestLte(old(pivots[..nchildren-1]), key);
-    //   //   assert key in old(children[llte+1].node.Interpretation());
-    //   //   assert old(children[llte+1].node.Interpretation()[key]) == old(Interpretation()[key]);
-    //   //   if llte < childidx as int {
-    //   //     assert key in Interpretation() && Interpretation()[key] == old(Interpretation()[key]);
-    //   //   } else if llte == childidx as int {
-    //   //     if Keys.lt(key, pivot) {
-    //   //       assert key in Interpretation() && Interpretation()[key] == old(Interpretation()[key]);
-    //   //     } else {
-    //   //       assert key in Interpretation() && Interpretation()[key] == old(Interpretation()[key]);
-    //   //     }
-    //   //   } else {
-    //   //     assert key in Interpretation() && Interpretation()[key] == old(Interpretation()[key]);
-    //   //   }
-    //   // }
-    //   // forall key | key in Interpretation()
-    //   //   ensures key in old(Interpretation()) && Interpretation()[key] == old(Interpretation()[key])
-    //   // {
-    //   //   var llte: int := Keys.LargestLte(pivots[..nchildren-1], key);
-    //   //   if llte < childidx as int {
-    //   //   } else if llte == childidx as int {
-    //   //   } else if llte == childidx as int + 1 {
-    //   //   } else {
-    //   //   }
-    //   // }
-    // }
-    
-    // function UnionSubtreeObjects() : set<object>
-    //   requires nchildren as int <= children.Length
-    //   requires forall i :: 0 <= i < nchildren ==> children[i].node != null
-    //   reads this, children, set i | 0 <= i < nchildren :: children[i].node
-    // {
-    //   set o, i | 0 <= i < nchildren && o in children[i].node.subtreeObjects :: o
-    // }
-    
-    // method Split() returns (pivot: Key, rightnode: Node)
-    //   requires WF()
-    //   requires Full()
-    //   ensures WF()
-    //   ensures rightnode.WF()
-    //   ensures SplitNode(old(ToImmutableNode()), ToImmutableNode(), rightnode.ToImmutableNode(), pivot)
-    //   ensures !Full()
-    //   ensures !rightnode.Full()
-    //   ensures subtreeObjects <= old(subtreeObjects)
-    //   ensures subtreeObjects !! rightnode.subtreeObjects
-    //   ensures fresh(rightnode.subtreeObjects - old(subtreeObjects))
-    //   modifies this      
-    // {
-    //   var right := new Index();
-    //   var boundary := nchildren/2;
-    //   Arrays.Memcpy(right.pivots, 0, pivots[boundary..nchildren-1]); // FIXME: remove conversion to seq
-    //   Arrays.Memcpy(right.children, 0, children[boundary..nchildren]); // FIXME: remove conversion to seq
-    //   right.nchildren := nchildren - boundary;
-    //   nchildren := boundary;
-    //   subtreeObjects := {this, pivots, children} + UnionSubtreeObjects();
-    //   right.subtreeObjects := right.subtreeObjects + right.UnionSubtreeObjects();
-
-    //   pivot := pivots[boundary-1];
-
-    //   rightnode := right;
-      
-    //   // Keys.reveal_IsStrictlySorted();
-    //   // assert WF();
-    //   // assert rightnode.WF();
-    //   // assert MergeMaps(Interpretation(), pivot, rightnode.Interpretation()) == old(Interpretation());
-    // }
-
-    // // method Insert(key: Key, value: Value)
-    // //   requires WF()
-    // //   requires !Full()
-    // //   ensures WF()
-    // //   ensures Interpretation() == old(Interpretation())[key := value]
-    // //   ensures allKeys == old(allKeys) + {key}
-    // //   ensures fresh(subtreeObjects - old(subtreeObjects))
-    // //   modifies this, subtreeObjects
-    // //   decreases allKeys
-    // // {
-    // //   var posplus1 := Keys.ArrayLargestLtePlus1(pivots, 0, nchildren - 1, key);
-    // //   var childidx := (posplus1) as uint64;
-    // //   if children[posplus1].node.Full() {
-    // //     childidx := SplitChild(key, childidx);
-    // //   }
-    // //   //AllKeysStrictlyDecreasing();
-    // //   children[childidx].node.Insert(key, value);
-    // //   subtreeObjects := subtreeObjects + children[childidx].node.subtreeObjects;
-    // //   allKeys := allKeys + {key};
-    // //   forall key' | key' in old(Interpretation()) && key' != key
-    // //     ensures key' in Interpretation() && Interpretation()[key'] == old(Interpretation()[key'])
-    // //   {
-    // //     var i :| 0 <= i < old(nchildren) && key' in old(children[i].node.Interpretation());
-    // //   }
-      
-    // // }
-
-    // constructor()
-    //   ensures nchildren == 0
-    //   ensures pivots.Length == (MaxChildren() as int)-1
-    //   ensures children.Length == (MaxChildren() as int)
-    //   ensures forall i :: 0 <= i < children.Length ==> children[i].node == null
-    //   ensures subtreeObjects == {this, pivots, children}
-    //   ensures fresh(pivots)
-    //   ensures fresh(children)
-    // {
-    //   pivots := new Key[MaxChildren()-1](_ => DefaultKey());
-    //   children := new NodeBox[MaxChildren()](_ => NodeBox(null));
-    //   nchildren := 0;
-    //   subtreeObjects := {this, pivots, children};
-    // }
-  }
-
-  // class MutableBtree {
-  //   var root: Node
-
-  //   function Interpretation() : map<Key, Value>
-  //     requires root.WF()
-  //     reads this, root, root.subtreeObjects
-  //   {
-  //     root.Interpretation()
-  //   }
-
-  //   method Query(needle: Key) returns (result: QueryResult)
-  //     requires root.WF()
-  //     ensures result == NotFound ==> needle !in Interpretation()
-  //     ensures result.Found? ==> needle in Interpretation() && Interpretation()[needle] == result.value
-  //   {
-  //     result := root.Query(needle);
-  //   }
-
-  //   method Insert(key: Key, value: Value)
-  //     requires root.WF()
-  //     ensures root.WF()
-  //     ensures Interpretation() == old(Interpretation())[key := value]
-  //     modifies this, root, root.subtreeObjects
-  //   {
-  //     if root.Full() {
-  //       var newroot := new Index();
-  //       newroot.children[0] := NodeBox(root);
-  //       newroot.nchildren := 1;
-  //       newroot.subtreeObjects := newroot.subtreeObjects + root.subtreeObjects;
-  //       newroot.allKeys := root.allKeys;
-  //       root := newroot;
-  //     }
-  //     AssumeFalse();
-  //     root.Insert(key, value);
-  //   }
-    
-  //   constructor()
-  //     ensures root.WF()
-  //     ensures Interpretation() == map[]
-  //   {
-  //     root := new Leaf();
-  //   }
+  // predicate method Full()
+  //   requires WF()
+  //   reads this, subtreeObjects
+  // {
+  //   nchildren == MaxChildren()
   // }
+
+  //   // predicate method Full()
+  //   //   requires WF()
+  //   //   reads this, subtreeObjects
+  //   // {
+  //   //   nkeys >= MaxKeysPerLeaf()
+  //   // }
+    
+  //   // method Split() returns (pivot: Key, rightnode: Node)
+  //   //   requires WF()
+  //   //   requires Full()
+  //   //   ensures WF()
+  //   //   ensures rightnode.WF()
+  //   //   ensures SplitNode(old(ToImmutableNode()), ToImmutableNode(), rightnode.ToImmutableNode(), pivot)
+  //   //   ensures !Full()
+  //   //   ensures !rightnode.Full()
+  //   //   ensures subtreeObjects <= old(subtreeObjects)
+  //   //   ensures subtreeObjects !! rightnode.subtreeObjects
+  //   //   ensures fresh(rightnode.subtreeObjects - old(subtreeObjects))
+  //   //   modifies this
+  //   // {
+  //   //   var right := new Leaf();
+  //   //   var boundary := nkeys/2;
+  //   //   Arrays.Memcpy(right.keys, 0, keys[boundary..nkeys]); // FIXME: remove conversion to seq
+  //   //   Arrays.Memcpy(right.values, 0, values[boundary..nkeys]); // FIXME: remove conversion to seq
+  //   //   right.nkeys := nkeys - boundary;
+  //   //   nkeys := boundary;
+  //   //   pivot := right.keys[0];
+  //   //   rightnode := right;
+
+  //   //   assert keys[..nkeys] == old(keys[..nkeys])[..nkeys];
+  //   //   Keys.StrictlySortedSubsequence(old(keys[..nkeys]), 0, nkeys as int);
+  //   //   assert right.keys[..right.nkeys] == old(keys[..nkeys])[boundary..old(nkeys)];
+  //   //   Keys.StrictlySortedSubsequence(old(keys[..nkeys]), boundary as int, old(nkeys) as int);
+  //   //   Keys.reveal_IsStrictlySorted();
+  //   //   assert SplitLeaf(old(ToImmutableNode()), ToImmutableNode(), rightnode.ToImmutableNode(), pivot);
+  //   // }
+      
+  //   // method Insert(key: Key, value: Value)
+  //   //   requires WF()
+  //   //   requires !Full()
+  //   //   ensures WF()
+  //   //   ensures Interpretation() == old(Interpretation())[key := value]
+  //   //   ensures AllKeys() == old(AllKeys()) + {key}
+  //   //   ensures fresh(subtreeObjects-old(subtreeObjects))
+  //   //   modifies this, subtreeObjects
+  //   //   decreases AllKeys()
+  //   // {
+  //   //   var posplus1 := Keys.ArrayLargestLtePlus1(keys, 0, nkeys, key);
+
+  //   //   if 1 <= posplus1 && keys[posplus1-1] == key {
+  //   //     values[posplus1-1] := value;
+  //   //   } else {
+  //   //     ghost var oldkeys := keys[..nkeys];
+  //   //     Arrays.Insert(keys, nkeys, key, posplus1);
+  //   //     Arrays.Insert(values, nkeys, value, posplus1);
+  //   //     nkeys := nkeys + 1;
+
+  //   //     InsertMultiset(oldkeys, key, posplus1 as int); // OBSERVE
+  //   //     Keys.strictlySortedInsert(oldkeys, key, posplus1 as int - 1); // OBSERVE
+  //   //     Keys.PosEqLargestLte(keys[..nkeys], key, posplus1 as int);
+  //   //     forall key' |  key' != key && key' in old(Interpretation())
+  //   //       ensures key' in Interpretation() && Interpretation()[key'] == old(Interpretation())[key']
+  //   //     {
+  //   //       var i: int := Keys.LargestLte(old(keys[..nkeys]), key');
+  //   //       //assert 0 <= i;
+  //   //       if i < posplus1 as int {
+  //   //         //assert keys[i] == key';
+  //   //         Keys.PosEqLargestLte(keys[..nkeys], key', i);
+  //   //       } else {
+  //   //         //assert keys[i+1] == key';
+  //   //         Keys.PosEqLargestLte(keys[..nkeys], key', i+1);
+  //   //       }
+  //   //     }
+  //   //     forall key' | key' != key && key' in Interpretation()
+  //   //       ensures key' in old(Interpretation()) && old(Interpretation())[key'] == Interpretation()[key']
+  //   //     {
+  //   //       var i: int := Keys.LargestLte(keys[..nkeys], key');
+  //   //       if i < posplus1 as int {
+  //   //         Keys.PosEqLargestLte(old(keys[..nkeys]), key', i);
+  //   //       } else {
+  //   //         Keys.PosEqLargestLte(old(keys[..nkeys]), key', i-1);
+  //   //       }
+  //   //     }
+  //   //   }
+  //   // }
+
+  //   // constructor()
+  //   //   ensures WF()
+  //   //   ensures Interpretation() == map[]
+  //   //   ensures !Full()
+  //   //   ensures fresh(keys)
+  //   //   ensures fresh(values)
+  //   // {
+  //   //   nkeys := 0;
+  //   //   keys := new Key[MaxKeysPerLeaf()](_ => DefaultKey());
+  //   //   values := new Value[MaxKeysPerLeaf()](_ => DefaultValue());
+  //   //   subtreeObjects := {this, keys, values};
+  //   // }
+  // }
+
+  // class Index extends Node {
+  //   var nchildren: uint64
+  //   var pivots: array<Key>
+  //   var children: array<NodeBox>
+
+
+  //   // lemma AllKeysStrictlyDecreasing()
+  //   //   requires WF()
+  //   //   ensures forall i :: 0 <= i < nchildren ==> children[i].node.allKeys < allKeys
+  //   // {
+  //   //   forall i | 0 <= i < nchildren
+  //   //     ensures children[i].node.allKeys < allKeys
+  //   //   {
+  //   //     var i' := if i < nchildren-1 then i+1 else 0;
+  //   //     assert i' != i;
+  //   //     assert children[i].node.allKeys !! children[i'].node.allKeys;
+  //   //     assert children[i].node.allKeys <= 
+  //   //     assert children[i].node.allKeys <= allKeys;
+  //   //   }
+  //   // }
+    
+  //   // method SplitChild(key: Key, childidx: uint64)
+  //   //   requires WF()
+  //   //   requires !Full()
+  //   //   requires childidx as int == 1 + Keys.LargestLte(pivots[..nchildren-1], key)
+  //   //   requires children[childidx].node.Full()
+  //   //   ensures WF()
+  //   //   //ensures Interpretation() == old(Interpretation())
+  //   //   ensures SplitChildOfIndex(old(ToImmutableNode()), ToImmutableNode(), childidx as int)
+  //   //   ensures fresh(subtreeObjects-old(subtreeObjects))
+  //   //   modifies this, pivots, children, children[childidx].node
+  //   // {
+  //   //   ghost var oldchildren := children;
+      
+  //   //   var pivot, right := children[childidx].node.Split();
+  //   //   Arrays.Insert(pivots, nchildren - 1, pivot, childidx);
+  //   //   Arrays.Insert(children, nchildren, NodeBox(right), childidx + 1);
+  //   //   nchildren := nchildren + 1;
+  //   //   subtreeObjects := subtreeObjects + right.subtreeObjects;
+
+      
+  //   //   // Keys.LargestLteIsUnique(old(pivots[..nchildren-1]), pivot, childidx as int - 1);
+  //   //   // Keys.strictlySortedInsert(old(pivots[..nchildren-1]), pivot, childidx as int - 1);
+
+  //   //   assert forall i: uint64 :: 0 <= i < childidx ==> children[i] == oldchildren[i];
+  //   //   assert children[childidx as int + 1].node == right;
+  //   //   assert forall i: uint64 :: childidx + 1 < i < nchildren ==> children[i] == oldchildren[i-1];
+  //   //   // forall i: int, j: int {:trigger children[i].node.subtreeObjects, children[j].node.subtreeObjects}
+  //   //   // | 0 <= i < j < nchildren as int
+  //   //   //   ensures children[i].node.subtreeObjects !! children[j].node.subtreeObjects
+  //   //   // {
+  //   //   //   if                                   j  < childidx as int {
+  //   //   //   } else if                            j == childidx as int {
+  //   //   //   } else if i  < childidx as int     && j == childidx as int + 1 {
+  //   //   //   } else if i == childidx as int     && j == childidx as int + 1 {
+  //   //   //   } else if i  < childidx as int     && j  > childidx as int + 1 {
+  //   //   //   } else if i == childidx as int     && j  > childidx as int + 1 {
+  //   //   //   } else if i == childidx as int + 1 && j  > childidx as int + 1 {
+  //   //   //   } else {
+  //   //   //   }
+  //   //   // }
+  //   //   // // forall i: int, key | 0 <= i < (nchildren as int)-1 && key in children[i].node.allKeys
+  //   //   // //   ensures Keys.lt(key, pivots[i])
+  //   //   // // {
+  //   //   // //   if childidx as int + 1 < i {
+  //   //   // //     assert children[i] == old(children[i-1]);
+  //   //   // //   }
+  //   //   // // }
+  //   //   // // forall i: int, key | 0 < i < nchildren as int && key in children[i].node.allKeys
+  //   //   // //   ensures Keys.lt(pivots[i-1], key)
+  //   //   // // {
+  //   //   // //   if i < childidx as int {
+  //   //   // //     assert Keys.lt(pivots[i-1], key);
+  //   //   // //   } else if i == childidx as int {
+  //   //   // //     assert Keys.lt(pivots[i-1], key);
+  //   //   // //   } else if i == childidx as int + 1 {
+  //   //   // //     assert Keys.lt(pivots[i-1], key);
+  //   //   // //   } else {
+  //   //   // //     assert Keys.lt(pivots[i-1], key);
+  //   //   // //   }
+  //   //   // // }
+  //   //   // assert WF();
+        
+  //   //   // forall key | key in old(Interpretation())
+  //   //   //   ensures key in Interpretation() && Interpretation()[key] == old(Interpretation()[key])
+  //   //   // {
+  //   //   //   var llte: int := Keys.LargestLte(old(pivots[..nchildren-1]), key);
+  //   //   //   assert key in old(children[llte+1].node.Interpretation());
+  //   //   //   assert old(children[llte+1].node.Interpretation()[key]) == old(Interpretation()[key]);
+  //   //   //   if llte < childidx as int {
+  //   //   //     assert key in Interpretation() && Interpretation()[key] == old(Interpretation()[key]);
+  //   //   //   } else if llte == childidx as int {
+  //   //   //     if Keys.lt(key, pivot) {
+  //   //   //       assert key in Interpretation() && Interpretation()[key] == old(Interpretation()[key]);
+  //   //   //     } else {
+  //   //   //       assert key in Interpretation() && Interpretation()[key] == old(Interpretation()[key]);
+  //   //   //     }
+  //   //   //   } else {
+  //   //   //     assert key in Interpretation() && Interpretation()[key] == old(Interpretation()[key]);
+  //   //   //   }
+  //   //   // }
+  //   //   // forall key | key in Interpretation()
+  //   //   //   ensures key in old(Interpretation()) && Interpretation()[key] == old(Interpretation()[key])
+  //   //   // {
+  //   //   //   var llte: int := Keys.LargestLte(pivots[..nchildren-1], key);
+  //   //   //   if llte < childidx as int {
+  //   //   //   } else if llte == childidx as int {
+  //   //   //   } else if llte == childidx as int + 1 {
+  //   //   //   } else {
+  //   //   //   }
+  //   //   // }
+  //   // }
+    
+  //   // function UnionSubtreeObjects() : set<object>
+  //   //   requires nchildren as int <= children.Length
+  //   //   requires forall i :: 0 <= i < nchildren ==> children[i].node != null
+  //   //   reads this, children, set i | 0 <= i < nchildren :: children[i].node
+  //   // {
+  //   //   set o, i | 0 <= i < nchildren && o in children[i].node.subtreeObjects :: o
+  //   // }
+    
+  //   // method Split() returns (pivot: Key, rightnode: Node)
+  //   //   requires WF()
+  //   //   requires Full()
+  //   //   ensures WF()
+  //   //   ensures rightnode.WF()
+  //   //   ensures SplitNode(old(ToImmutableNode()), ToImmutableNode(), rightnode.ToImmutableNode(), pivot)
+  //   //   ensures !Full()
+  //   //   ensures !rightnode.Full()
+  //   //   ensures subtreeObjects <= old(subtreeObjects)
+  //   //   ensures subtreeObjects !! rightnode.subtreeObjects
+  //   //   ensures fresh(rightnode.subtreeObjects - old(subtreeObjects))
+  //   //   modifies this      
+  //   // {
+  //   //   var right := new Index();
+  //   //   var boundary := nchildren/2;
+  //   //   Arrays.Memcpy(right.pivots, 0, pivots[boundary..nchildren-1]); // FIXME: remove conversion to seq
+  //   //   Arrays.Memcpy(right.children, 0, children[boundary..nchildren]); // FIXME: remove conversion to seq
+  //   //   right.nchildren := nchildren - boundary;
+  //   //   nchildren := boundary;
+  //   //   subtreeObjects := {this, pivots, children} + UnionSubtreeObjects();
+  //   //   right.subtreeObjects := right.subtreeObjects + right.UnionSubtreeObjects();
+
+  //   //   pivot := pivots[boundary-1];
+
+  //   //   rightnode := right;
+      
+  //   //   // Keys.reveal_IsStrictlySorted();
+  //   //   // assert WF();
+  //   //   // assert rightnode.WF();
+  //   //   // assert MergeMaps(Interpretation(), pivot, rightnode.Interpretation()) == old(Interpretation());
+  //   // }
+
+  //   // // method Insert(key: Key, value: Value)
+  //   // //   requires WF()
+  //   // //   requires !Full()
+  //   // //   ensures WF()
+  //   // //   ensures Interpretation() == old(Interpretation())[key := value]
+  //   // //   ensures allKeys == old(allKeys) + {key}
+  //   // //   ensures fresh(subtreeObjects - old(subtreeObjects))
+  //   // //   modifies this, subtreeObjects
+  //   // //   decreases allKeys
+  //   // // {
+  //   // //   var posplus1 := Keys.ArrayLargestLtePlus1(pivots, 0, nchildren - 1, key);
+  //   // //   var childidx := (posplus1) as uint64;
+  //   // //   if children[posplus1].node.Full() {
+  //   // //     childidx := SplitChild(key, childidx);
+  //   // //   }
+  //   // //   //AllKeysStrictlyDecreasing();
+  //   // //   children[childidx].node.Insert(key, value);
+  //   // //   subtreeObjects := subtreeObjects + children[childidx].node.subtreeObjects;
+  //   // //   allKeys := allKeys + {key};
+  //   // //   forall key' | key' in old(Interpretation()) && key' != key
+  //   // //     ensures key' in Interpretation() && Interpretation()[key'] == old(Interpretation()[key'])
+  //   // //   {
+  //   // //     var i :| 0 <= i < old(nchildren) && key' in old(children[i].node.Interpretation());
+  //   // //   }
+      
+  //   // // }
+
+  //   // constructor()
+  //   //   ensures nchildren == 0
+  //   //   ensures pivots.Length == (MaxChildren() as int)-1
+  //   //   ensures children.Length == (MaxChildren() as int)
+  //   //   ensures forall i :: 0 <= i < children.Length ==> children[i].node == null
+  //   //   ensures subtreeObjects == {this, pivots, children}
+  //   //   ensures fresh(pivots)
+  //   //   ensures fresh(children)
+  //   // {
+  //   //   pivots := new Key[MaxChildren()-1](_ => DefaultKey());
+  //   //   children := new NodeBox[MaxChildren()](_ => NodeBox(null));
+  //   //   nchildren := 0;
+  //   //   subtreeObjects := {this, pivots, children};
+  //   // }
+  // }
+
+  // // class MutableBtree {
+  // //   var root: Node
+
+  // //   function Interpretation() : map<Key, Value>
+  // //     requires root.WF()
+  // //     reads this, root, root.subtreeObjects
+  // //   {
+  // //     root.Interpretation()
+  // //   }
+
+  // //   method Query(needle: Key) returns (result: QueryResult)
+  // //     requires root.WF()
+  // //     ensures result == NotFound ==> needle !in Interpretation()
+  // //     ensures result.Found? ==> needle in Interpretation() && Interpretation()[needle] == result.value
+  // //   {
+  // //     result := root.Query(needle);
+  // //   }
+
+  // //   method Insert(key: Key, value: Value)
+  // //     requires root.WF()
+  // //     ensures root.WF()
+  // //     ensures Interpretation() == old(Interpretation())[key := value]
+  // //     modifies this, root, root.subtreeObjects
+  // //   {
+  // //     if root.Full() {
+  // //       var newroot := new Index();
+  // //       newroot.children[0] := NodeBox(root);
+  // //       newroot.nchildren := 1;
+  // //       newroot.subtreeObjects := newroot.subtreeObjects + root.subtreeObjects;
+  // //       newroot.allKeys := root.allKeys;
+  // //       root := newroot;
+  // //     }
+  // //     AssumeFalse();
+  // //     root.Insert(key, value);
+  // //   }
+    
+  // //   constructor()
+  // //     ensures root.WF()
+  // //     ensures Interpretation() == map[]
+  // //   {
+  // //     root := new Leaf();
+  // //   }
+  // // }
 }
 
-// module TestMutableBtree refines MutableBtree {
-//   import Keys = Uint64_Order
-//   type Value = uint64
+module TestBtreeSpec refines BtreeSpec {
+  import Keys = Integer_Order
+  type Value = int
+}
 
-//   function method MaxKeysPerLeaf() : uint64 { 64 }
-//   function method MaxChildren() : uint64 { 64 }
+module TestMutableBtree refines MutableBtree {
+  import BS = TestBtreeSpec
+    
+  function method MaxKeysPerLeaf() : uint64 { 64 }
+  function method MaxChildren() : uint64 { 64 }
 
-//   function method DefaultValue() : Value { 0 }
-//   function method DefaultKey() : Key { 0 }
-// }
+  function method DefaultValue() : Value { 0 }
+  function method DefaultKey() : Key { 0 }
+}
 
 // module MainModule {
 //   import opened NativeTypes
